close admitted struct deinit lemma

theories/rust_typing/struct/deinit.v
@@ -1,6 +1,7 @@
 From refinedrust Require Export base type ltypes.
 From refinedrust Require Import ltype_rules.
-From refinedrust Require Import programs struct.subltype.
+From refinedrust Require Import programs uninit.
+From refinedrust.struct Require Import subltype unfold.
 From refinedrust Require Import options.
 
 (** ** Lemmas about deinitializing *)
@@ -8,54 +9,88 @@ From refinedrust Require Import options.
 Section deinit.
   Context `{!typeGS Σ}.
 
+  Fixpoint uninit_tys (ls : list syn_type) : hlist type (replicate (length ls) (unit : Type)) :=
+    match ls with
+    | [] => +[]
+    | st :: sts =>
+        uninit st +:: uninit_tys sts
+    end.
+  Lemma uninit_tys_lookup_inv (sts : list syn_type) k x :
+    hzipl _ (uninit_tys sts) !! k = Some x →
+    ∃ st, sts !! k = Some st ∧ x = existT (unit : Type) (uninit st).
+  Proof.
+    induction sts as [ | st sts IH] in k, x |-*; simpl; first done.
+    destruct k as [ | k]; simpl.
+    - intros [= <-]. eauto.
+    - apply IH.
+  Qed.
 
-  (* TODO *)
-  Lemma ltype_deinit_struct F π {rts} (lts : hlist ltype rts) (sls : struct_layout_spec) rs st l wl :
+  Fixpoint uninit_rs (ls : list syn_type) : plist id (replicate (length ls) (unit : Type)) :=
+    match ls with
+    | [] => *[]
+    | st :: sts =>
+        tt *:: uninit_rs sts
+    end.
+  Lemma uninit_rs_lookup_inv (sts : list syn_type) k x :
+    pzipl _ (uninit_rs sts) !! k = Some x →
+    ∃ st, sts !! k = Some st ∧ x = existT (unit : Type) tt.
+  Proof.
+    induction sts as [ | st sts IH] in k, x |-*; simpl; first done.
+    destruct k as [ | k]; simpl.
+    - intros [= <-]. eauto.
+    - apply IH.
+  Qed.
+
+  Lemma ltype_deinit_struct F π (sls : struct_layout_spec) rs st l wl :
     lftE ⊆ F →
     syn_type_compat sls st →
-    (l ◁ₗ[π, Owned wl] rs @ (StructLtype lts sls)) ={F}=∗
+    (l ◁ₗ[π, Owned wl] (#rs) @ (StructLtype (hmap (@OfTy _ _) (uninit_tys (sls_fields sls).*2)) sls)) ={F}=∗
     l ◁ₗ[π, Owned false] #() @ (◁ uninit st).
   Proof.
     iIntros (? Hstcomp) "Hl".
-    rewrite ltype_own_struct_unfold /struct_ltype_own.
-    (* this doesn't hold because we might have an alias. *)
+    iPoseProof (struct_t_unfold_2_owned) as "#Ha".
+    iMod (fupd_mask_subseteq lftE) as "Hcl"; first done.
+    iMod ("Ha" with "Hl") as "Hl".
+    iMod "Hcl" as "_". iClear "Ha".
+    iMod (ltype_own_Owned_to_false with "Hl") as "Hl"; first done.
 
-    (*
-    iDestruct "Hl" as "(%ly & %Halg & % & Hlb & Hcreds & %r' & ? & Hb)".
-    iMod (maybe_use_credit with "Hcreds Hb") as "(? & ? & %l' & Hl & Hb)"; first done.
-    rewrite ltype_own_ofty_unfold /lty_of_ty_own.
-    iModIntro. iExists ly. simpl. iSplitR.
-    { destruct Hstcomp as [<- | (ly1 & Hst' & ->)]; first done.
-      simpl. iPureIntro. eapply syn_type_has_layout_make_untyped; last done.
-      by eapply syn_type_has_layout_inj. }
-    iR. iR.
-    iSplitL "Hlb"; first by iFrame. iR.
-    iExists tt. iR.
-    iModIntro. iExists l'. iFrame. rewrite uninit_own_spec. iExists ly.
-    apply syn_type_has_layout_ptr_inv in Halg as ->. iSplitR; last done.
-    iPureIntro. destruct Hstcomp as [<- | (ly1 & Hst' & ->)]; first done.
-    specialize (syn_type_has_layout_ptr_inv _ Hst') as ->.
-    eapply syn_type_has_layout_make_untyped; done.
+    iPoseProof (ltype_own_has_layout with "Hl") as "(%ly & %Halg & %Hl)".
+    simp_ltypes in Halg. simpl in Halg.
+    iApply (ofty_owned_subtype_aligned with "[] Hl"); [ | done | ].
+    { destruct Hstcomp as [<- | Hst]; first done.
+      destruct Hst as (ly1 & Hst & ->). simpl.
+      specialize (syn_type_has_layout_inj _ _ _ Hst Halg) as ->.
+      by eapply syn_type_has_layout_make_untyped. }
+    iApply (owned_type_incl_uninit' _ _ _ _ _ ly); simpl.
+    - destruct Hstcomp as [<- | Hst]; first apply syn_type_size_eq_refl.
+      destruct Hst as (ly1 & Hst & ->). simpl.
+      specialize (syn_type_has_layout_inj _ _ _ Hst Halg) as ->.
+      intros ly1 ly2 Halg1 Halg2.
+      specialize (syn_type_has_layout_inj _ _ _ Hst Halg1) as ->.
+      apply syn_type_has_layout_untyped_inv in Halg2 as (-> & _); done.
+    - destruct Hstcomp as [<- | Hst]; first done.
+      destruct Hst as (ly1 & Hst & ->).
+      specialize (syn_type_has_layout_inj _ _ _ Hst Halg) as ->.
+      by eapply syn_type_has_layout_make_untyped.
   Qed.
-     *)
-  Abort.
-
 End deinit.
 
 Section rules.
-  Context `{!typeGS Σ}.
+Context `{!typeGS Σ}.
+
 
   (* We iterate over all the fields to deinitialize them first, and then deinitialize the struct itself *)
-  Lemma owned_subltype_step_struct_uninit π E L l {rts} (lts : hlist ltype rts) rs sls st T :
+  Lemma owned_subltype_step_struct_uninit π E L l {rts} (lts : hlist ltype rts) rs (sls : struct_layout_spec) (st : syn_type) T :
     owned_subltype_step π E L l #rs #() (StructLtype lts sls) (◁ uninit st) T :-
-    exhale (⌜st = sls⌝);
+    exhale (⌜syn_type_compat sls st⌝);
     L2, R2 ← iterate: zip (hpzipl rts lts rs) sls.(sls_fields) with L, True%I {{ '((existT rt (lt, r)), (field, stf)) T L2 R2,
+      exhale (⌜ltype_st lt = stf⌝);
       return owned_subltype_step π E L2 (l atst{sls}ₗ field) r #() lt (◁ uninit stf) (λ L3 R3,
         T L3 (R2 ∗ R3))
       }};
     return T L2 R2.
   Proof.
-    iIntros "(-> & Hit)".
+    iIntros "(%Hcomp & Hit)".
     iIntros (??) "#CTX #HE HL Hl".
 
     rewrite ltype_own_struct_unfold/struct_ltype_own/=.
@@ -63,21 +98,124 @@ Section rules.
     iMod (fupd_mask_mono with "Hl") as "Hl"; first done.
 
     iPoseProof (struct_ltype_focus_components with "Hl") as "(Hl & Hclose_l)"; [done.. | ].
-    (*Search li.iterate "elim".*)
-    (* invariant: ownership of the first n uninit segments.
-        ownership for the rest
-    *)
 
-    (*
-    set (INV := λ (i : nat) (L2 : llctx) (R2 : iProp Σ),
+    set (INV := (λ (idx : nat) (L2 : llctx) (R2 : iProp Σ),
       llctx_interp L2 ∗
+      ([∗ list] i↦'(existT rt (lt, r)) ∈ hpzipl rts lts rs',
+          if decide (idx ≤ i) then
+          ∃ (name : string) (st : syn_type), ⌜sls_fields sls !! i = Some (name, st)⌝ ∗ l atst{sls}ₗ name ◁ₗ[ π, Owned false] r @ lt
+          else True) ∗
+      logical_step F (R2 ∗
+        ([∗ list] i↦'(existT rt (lt, r)) ∈ hpzipl rts lts rs',
+          if decide (i < idx) then
+          ∃ (name : string) (st : syn_type),
+          ⌜sls_fields sls !! i = Some (name, st)⌝ ∗
+          ⌜ltype_st lt = st⌝ ∗
+          l atst{sls}ₗ name ◁ₗ[ π, Owned false] #() @ ◁ uninit (ltype_st lt)
+          else True)
+      ))%I).
 
-      logical_step F ( ∗ R2)).
-     *)
+    iMod (iterate_elim2_fupd INV with "Hit [Hl HL] []") as "(%L2 & %R2 & Hinv & HT)".
+    { (* initialization *)
+      unfold INV. iFrame. iApply logical_step_intro.
+      iR. simpl. iApply big_sepL_intro.
+      iIntros "!>" (? [? []] ?). done. }
+    { (* preservation *)
+      iModIntro. iIntros (i [[rt [lt r']] [name st']] T' L2 R2 Hlook) "Hinv Hsub".
+      iDestruct "Hinv" as "(HL & Hinv & Hstep)".
 
-    (*Search iterate_elim2*)
+      apply lookup_zip in Hlook as [Hlook1 Hlook2].
+      iPoseProof (big_sepL_delete with "Hinv") as "(Ha & Hinv)"; first apply Hlook1.
+      simpl. rewrite decide_True; last lia.
+      iDestruct "Ha" as "(% & % & %Hlook2' & Ha)".
+      rewrite Hlook2 in Hlook2'. injection Hlook2' as <- <-.
+      iDestruct "Hsub" as "(<- & Hsub)".
+      iMod ("Hsub" with "[] CTX HE HL Ha") as "(%L3 & %R3 & Hs & %Hst_eq & HL & HT)"; first done.
 
-  Admitted.
+      iModIntro. iExists _, _. iFrame.
+      iSplitL "Hinv".
+      { iApply (big_sepL_mono with "Hinv"). iIntros (? [? []] ?) "Ha".
+        repeat case_decide; try done; lia. }
+      iApply (logical_step_compose with "Hstep").
+      iApply (logical_step_wand with "Hs").
+      iIntros "(Ha & HR) (HR2 & Hb)". iFrame.
+      iEval (rewrite -(list_insert_id (hpzipl rts lts rs') i _ Hlook1)).
+      iApply big_sepL_insert.
+      { by apply lookup_lt_is_Some_1. }
+      simpl.
+      iSplitL "Ha".
+      { rewrite decide_True; last lia. eauto with iFrame. }
+      iApply (big_sepL_mono with "Hb"). iIntros (? [? []] ?) "Ha".
+      repeat case_decide; try done; lia. }
+    iDestruct "Hinv" as "(HL & _ & Hs)".
+    iModIntro. iExists _, _. iFrame.
+    iSplitL; first last.
+    { iPureIntro. simp_ltypes.
+      by eapply syn_type_compat_size_eq. }
+    iApply logical_step_fupd.
+    iApply (logical_step_wand with "Hs").
+    iIntros "(HR & Hx)". iFrame.
+    clear INV.
+
+    (* extract pure info from invariant *)
+    iAssert (⌜Forall2 (λ '(existT rt (lt, _)) st, ltype_st lt = st) (hpzipl rts lts rs') (sls_fields sls).*2⌝)%I with "[Hx]" as "%Hf".
+    { iApply big_sepL2_Forall2.
+      iPoseProof (big_sepL_extend_r with "Hx") as "Hx"; last iApply (big_sepL2_wand with "Hx").
+      { rewrite length_fmap length_hpzipl Hlen//. }
+      iApply big_sepL2_intro. { rewrite length_fmap length_hpzipl Hlen//. }
+      iIntros "!>" (? [? []] ? Hlook1 Hlook2).
+      apply list_lookup_fmap_Some in Hlook2 as ([name st'] & Hlook2 & ->).
+      rewrite decide_True; first last. { rewrite zip_length length_hpzipl Hlen.
+        apply hpzipl_lookup_inv in Hlook1. apply lookup_lt_Some in Hlook1. lia. }
+      iIntros "(% & % & %Hlook3 & <- & _)".
+      simplify_eq. done. }
+
+    set (lts' := (hmap (@OfTy _ _) (uninit_tys (sls_fields sls).*2))).
+    set (rs'' := (pmap (λ _ x, #x) (uninit_rs  (sls_fields sls).*2))).
+    iPoseProof ("Hclose_l" $! _ lts' rs'' with "[] [] [Hx]")as "Hx".
+    { iPureIntro. rewrite -Hlen length_replicate length_fmap//. }
+    { iPureIntro.
+      eapply (Forall2_transitive _ (λ st '(existT rt (lt, _)), st = ltype_st lt)); [ | apply Hf | ].
+      - intros [? []] st' [? []]; simpl. naive_solver.
+      - unfold lts', rs''.
+        generalize (sls_fields sls).*2 as sts.
+        clear. induction sts as [ | st sts IH]; simpl; first done.
+        econstructor; last done. simp_ltypes. done. }
+    { iApply big_sepL2_elim_r.
+      iPoseProof (big_sepL_extend_l with "Hx") as "Hx"; last iApply (big_sepL2_wand with "Hx").
+      { rewrite !length_hpzipl length_replicate length_fmap -Hlen//. }
+      iApply big_sepL2_intro.
+      { rewrite !length_hpzipl length_replicate length_fmap -Hlen//. }
+      iModIntro. iIntros (k [rt1 [lt1 rs1]] [rt2 [lt2 rs2]] Hlook1 Hlook2).
+
+      apply hpzipl_lookup_inv in Hlook1 as Hlook1'.
+      apply lookup_replicate_1 in Hlook1' as (-> & Hk).
+      rewrite length_fmap in Hk.
+      rewrite decide_True; first last. { rewrite zip_length length_hpzipl. lia. }
+
+      apply hpzipl_lookup_inv_hzipl_pzipl in Hlook1 as (Hlook1_1 & Hlook1_2).
+      subst lts'.
+      eapply hzipl_hmap_lookup_inv in Hlook1_1 as (ty & Hlook1_1 & ->).
+      apply uninit_tys_lookup_inv in Hlook1_1 as (st' & Hlook1_1 & Heq).
+      apply existT_inj in Heq as ->.
+
+      eapply pzipl_pmap_lookup_inv in Hlook1_2 as (ty & Hlook1_2 & ->).
+      apply uninit_rs_lookup_inv in Hlook1_2 as (st'' & Hlook1_2 & Heq).
+      apply existT_inj in Heq as ->.
+      rewrite Hlook1_1 in Hlook1_2. injection Hlook1_2 as [= <-].
+
+      iIntros "(%name & %st'' & %Hlook_fields & <- & Ha)".
+      iExists name, _. iR.
+      apply list_lookup_fmap_Some in Hlook1_1 as ([name' st''] & Hlook1_1 & ->).
+      simplify_eq. done. }
+    iApply (ltype_deinit_struct _ _ sls (rs'') _ _ false); first done.
+    { done. }
+
+    rewrite ltype_own_struct_unfold/struct_ltype_own.
+    iExists _. iR.
+    iSplitR. { rewrite length_replicate length_fmap//. }
+    iR. iFrame. iR. done.
+  Qed.
   Definition owned_subltype_step_struct_uninit_inst := [instance owned_subltype_step_struct_uninit].
   Global Existing Instance owned_subltype_step_struct_uninit_inst | 20.
 
